arm+arm-hyp machine: add omap3 machine options + operations
Make pptrBase configurable, add haveSetTrigger config, and
handleSpuriousIRQ machine op.

Configure pptrBase depending on config_PLAT_OMAP3. The omap3 platform
is the only AArch32 platform that has a different pptrBase, so it is
easier to define via an `if` here than trying to parse the value out of
a variety of C source headers.

Define haveSetTrigger to account for platforms that cannot set the IRQ
trigger. Not a CMake config option, which means it is not easy to
extract from kernel sources. Define the list of relevant platforms
manually instead.

Add handleSpuriousIRQ machine op for omap3 and am355x.

Technically, ARM_HYP is not configurable for omap3, am335x and bcm2837,
but the definitions in Haskell are shared with ARM, so it is nicer to
introduce them for ASpec as well and make the proofs generic. If there
ever is a non-GIC platform with hyp support, the proofs should then
work.

Signed-off-by: Gerwin Klein <gerwin.klein@proofcraft.systems>

spec/machine/ARM/Platform.thy
@@ -36,18 +36,37 @@ context Arch begin global_naming ARM
 value_type irq_len = Kernel_Config.irqBits (* IRQ_CNODE_SLOT_BITS *)
 type_synonym irq = "irq_len word"
 
+(* List of supported Arm platforms that support GICv3 or GICv2 *)
+definition isGICPlatform :: bool where
+  "isGICPlatform \<equiv> \<not>(config_PLAT_OMAP3 \<or> config_PLAT_AM335X \<or> config_PLAT_BCM2837)"
+
+lemmas Kernel_Config_isGICPlatform_def =
+  isGICPlatform_def
+  Kernel_Config.config_PLAT_OMAP3_def
+  Kernel_Config.config_PLAT_AM335X_def
+  Kernel_Config.config_PLAT_BCM2837_def
+
 (* Software-generated interrupts *)
 definition numSGIs_bits :: nat where
   "numSGIs_bits = 4"
 
 definition numSGIs :: nat where
-  "numSGIs = 2^numSGIs_bits"
+  "numSGIs \<equiv> if isGICPlatform then 2^numSGIs_bits else 0"
 
 definition gicNumTargets_bits :: nat where
   "gicNumTargets_bits \<equiv> if Kernel_Config.config_ARM_GIC_V3 then 4 else 3"
 
 definition gicNumTargets :: nat where
-  "gicNumTargets \<equiv> 2^gicNumTargets_bits"
+  "gicNumTargets \<equiv> if isGICPlatform then 2^gicNumTargets_bits else 0"
+
+(* Platforms that have a setTrigger IRQ function. These are currently all
+   platforms that support the Arm GIC. *)
+definition haveSetTrigger :: bool where
+  "haveSetTrigger \<equiv> isGICPlatform"
+
+lemmas Kernel_Config_haveSetTrigger_def =
+  haveSetTrigger_def
+  Kernel_Config_isGICPlatform_def
 
 end
 
@@ -76,9 +95,23 @@ definition cacheLineBits :: nat where
 definition cacheLine :: nat where
   "cacheLine = 2^cacheLineBits"
 
-(* The first virtual address of the kernel's physical memory window *)
+(* The first virtual address of the kernel's physical memory window.
+   Coincides with seL4_UserTop and USER_TOP in C for AArch32.
+
+   The definition below singles out the omap3 platform, because it is the only AArch32
+   platform that does not put seL4_UserTop at 0xe0000000. The macro definition in C is
+   hard to get at for the kernel config generation script and the definition here is
+   comparatively straightforward. *)
 definition pptrBase :: word32 where
-  "pptrBase \<equiv> 0xe0000000"
+  "pptrBase \<equiv> if config_PLAT_OMAP3 then 0xf0000000 else 0xe0000000"
+
+schematic_goal pptrBase_val:
+  "pptrBase = numeral ?n"
+  by (simp add: pptrBase_def Kernel_Config.config_PLAT_OMAP3_def del: word_eq_numeral_iff_iszero)
+
+lemma pptrBase_top_neq_0: (* 20 = size of ARMSectionBits *)
+  "pptrBase >> 20 \<noteq> 0"
+  by (simp add: pptrBase_def)
 
 abbreviation (input) "paddrBase \<equiv> physBase"
 
